ms chachapoly

code/api/Hacl.AEAD.Chacha20Poly1305.fst
@@ -1,5 +1,6 @@
 module Hacl.AEAD.Chacha20Poly1305
 
+open FStar.HyperStack
 open FStar.Buffer
 open FStar.ST
 open Hacl.Constants
@@ -23,74 +24,173 @@ let noncelen = 12
 let keylen = 32
 let maclen = 16
 
+
+#reset-options "--initial_fuel 0 --max_fuel 0 --z3rlimit 100"
+
+private val lemma_aead_encrypt_poly:
+  h0:mem -> h1:mem -> h2:mem -> h3:mem -> h4:mem ->
+  r:buffer Hacl.UInt64.t -> acc:buffer Hacl.UInt64.t -> mac:uint8_p ->
+  Lemma (requires (live h0 mac /\ ~(contains h0 r) /\ ~(contains h0 acc)
+    /\ live h1 mac /\ live h1 r /\ live h1 acc
+    /\ live h2 mac /\ live h2 r /\ live h2 acc
+    /\ live h3 mac /\ live h3 r /\ live h3 acc
+    /\ live h4 mac /\ live h4 r /\ live h4 acc
+    /\ modifies_0 h0 h1 /\ modifies_2 r acc h1 h2 /\ modifies_1 acc h2 h3 /\ modifies_2 mac acc h3 h4))
+        (ensures (modifies_2_1 mac h0 h4))
+private let lemma_aead_encrypt_poly h0 h1 h2 h3 h4 r acc mac =
+  lemma_reveal_modifies_0 h0 h1;
+  lemma_reveal_modifies_2 r acc h1 h2;
+  lemma_reveal_modifies_1 acc h2 h3;
+  lemma_reveal_modifies_2 mac acc h3 h4;
+  lemma_intro_modifies_2_1 mac h0 h4
+
+
 #reset-options "--initial_fuel 0 --max_fuel 0 --z3rlimit 50"
+
+private val aead_encrypt_poly:
+  c:uint8_p ->
+  mlen:u32{let len = U32.v mlen in len = length c}  ->
+  mac:uint8_p{length mac = maclen /\ disjoint mac c} ->
+  aad:uint8_p ->
+  aadlen:u32{let len = U32.v aadlen in len = length aad}  ->
+  k:uint8_p{length k = keylen /\ disjoint k mac} ->
+  n:uint8_p{length n = noncelen /\ disjoint n mac} ->
+  b:uint8_p{length b >= 80 /\ disjoint b mac} ->
+  Stack unit
+    (requires (fun h -> live h c /\ live h mac /\ live h n /\ live h k /\ live h aad /\ live h b))
+    (ensures  (fun h0 z h1 -> modifies_1 mac h0 h1 /\ live h1 mac))
+#reset-options "--initial_fuel 0 --max_fuel 0 --z3rlimit 100"
+private let aead_encrypt_poly  c mlen mac aad aadlen k n tmp =
+  let b = Buffer.sub tmp 0ul 64ul in
+  let lb = Buffer.sub tmp 64ul 16ul in
+  let mk = Buffer.sub b 0ul 32ul in
+  let key_s = Buffer.sub mk 16ul 16ul in
+  push_frame();
+  let h0 = ST.get() in
+  let st = Poly1305_64.alloc () in
+  let h1 = ST.get() in
+  let log = Poly1305_64.poly1305_blocks_init st aad aadlen mk in
+  let h2 = ST.get() in
+  let log = Poly1305_64.poly1305_blocks_continue log st c mlen in
+  let h3 = ST.get() in
+  let log = Poly1305_64.poly1305_blocks_finish log st lb mac key_s in
+  let h4 = ST.get() in
+  lemma_aead_encrypt_poly h0 h1 h2 h3 h4 Hacl.Impl.Poly1305_64.(st.r) Hacl.Impl.Poly1305_64.(st.h) mac;
+  pop_frame()
+
+
+
+private val lemma_aead_encrypt:
+  h0:mem -> h1:mem -> h2:mem -> h3:mem -> h4:mem ->
+  c:uint8_p -> b:uint8_p -> mac:uint8_p ->
+  Lemma (requires (live h0 c /\ live h0 mac /\ ~(contains h0 b)
+    /\ live h1 c /\ live h1 mac /\ live h1 b
+    /\ live h2 c /\ live h2 mac /\ live h2 b
+    /\ live h3 c /\ live h3 mac /\ live h3 b
+    /\ live h4 c /\ live h4 mac /\ live h4 b
+    /\ modifies_0 h0 h1 /\ modifies_1 c h1 h2 /\ modifies_1 b h2 h3 /\ modifies_1 mac h3 h4))
+        (ensures (modifies_3_2 c mac h0 h4))
+#reset-options "--initial_fuel 0 --max_fuel 0 --z3rlimit 100"
+private let lemma_aead_encrypt h0 h1 h2 h3 h4 c b mac =
+  lemma_reveal_modifies_0 h0 h1;
+  lemma_reveal_modifies_1 c h1 h2;
+  lemma_reveal_modifies_1 b h2 h3;
+  lemma_reveal_modifies_1 mac h3 h4;
+  lemma_intro_modifies_3_2 c mac h0 h4
+
 
 val aead_encrypt:
   c:uint8_p ->
   mac:uint8_p{length mac = maclen /\ disjoint mac c} ->
-  m:uint8_p ->
+  m:uint8_p{disjoint c m} ->
   mlen:u32{let len = U32.v mlen in len = length m /\ len = length c}  ->
   aad:uint8_p ->
   aadlen:u32{let len = U32.v aadlen in len = length aad}  ->
-  k:uint8_p{length k = keylen} ->
-  n:uint8_p{length n = noncelen} ->
+  k:uint8_p{length k = keylen /\ disjoint k mac /\ disjoint k c} ->
+  n:uint8_p{length n = noncelen /\ disjoint n mac /\ disjoint n c} ->
   Stack u32
-    (requires (fun h -> live h c /\ live h mac /\ live h m /\ live h n /\ live h k))
+    (requires (fun h -> live h c /\ live h mac /\ live h m /\ live h n /\ live h k /\ live h aad))
     (ensures  (fun h0 z h1 -> modifies_2 c mac h0 h1 /\ live h1 c /\ live h1 mac))
 let aead_encrypt c mac m mlen aad aadlen k n =
   push_frame();
-  Chacha20.chacha20 c m mlen k n 1ul;
-  let b = create (uint8_to_sint8 0uy) 64ul in
-  Chacha20.chacha20_key_block b k n 0ul;
-  let mk = Buffer.sub b 0ul 32ul in
-  let key_s = Buffer.sub mk 16ul 16ul in
-
-  let st = Poly1305_64.alloc () in
-  let lb = create (uint8_to_sint8 0uy) 16ul in
-  Poly1305_64.poly1305_blocks_init st aad aadlen mk;
-  Poly1305_64.poly1305_blocks_continue st c mlen;
+  let h0 = ST.get() in
+  let tmp = create (uint8_to_sint8 0uy) 80ul in
+  let b = Buffer.sub tmp 0ul 64ul in
+  let lb = Buffer.sub tmp 64ul 16ul in
   hstore64_le (Buffer.sub lb 0ul 8ul) (uint32_to_sint64 aadlen);
   hstore64_le (Buffer.sub lb 8ul 8ul) (uint32_to_sint64 mlen);
-  Poly1305_64.poly1305_blocks_finish st lb mac key_s;
+  let h1 = ST.get() in
+  cut (modifies_0 h0 h1);
+  Chacha20.chacha20 c m mlen k n 1ul;
+  let h2 = ST.get() in
+  Chacha20.chacha20_key_block b k n 0ul;
+  let h3 = ST.get() in
+  let mk = Buffer.sub b 0ul 32ul in
+  let key_s = Buffer.sub mk 16ul 16ul in
+  aead_encrypt_poly  c mlen mac aad aadlen k n tmp;
+  let h4 = ST.get() in
+  lemma_aead_encrypt h0 h1 h2 h3 h4 c tmp mac;
   pop_frame();
   0ul
 
 
 #reset-options "--initial_fuel 0 --max_fuel 0 --z3rlimit 200"
 
+private let lemma_aead_decrypt_ (h:mem) (h':mem) (m:uint8_p) : Lemma 
+  (h == h' ==> modifies_1 m h h')
+  = lemma_intro_modifies_1 m h h
+
+
+private val lemma_aead_decrypt:
+  h0:mem -> h1:mem -> h2:mem ->
+  tmp:uint8_p -> m:uint8_p ->
+  Lemma (requires (~(contains h0 tmp) /\ live h0 m /\ live h1 tmp /\ live h1 m /\ live h2 tmp /\ live h2 m
+    /\ modifies_0 h0 h1 /\ (modifies_1 m h1 h2 \/ h1 == h2)))
+        (ensures (modifies_2_1 m h0 h2))
+let lemma_aead_decrypt h0 h1 h2 tmp m =
+  lemma_reveal_modifies_0 h0 h1;
+  lemma_aead_decrypt_ h1 h2 m;
+  lemma_reveal_modifies_1 m h1 h2;
+  lemma_intro_modifies_2_1 m h0 h2
+
+
 val aead_decrypt:
   m:uint8_p ->
-  c:uint8_p ->
+  c:uint8_p{disjoint m c} ->
   mlen:u32{let len = U32.v mlen in len = length m /\ len = length c}  ->
-  mac:uint8_p{length mac = maclen /\ disjoint mac c} ->
+  mac:uint8_p{length mac = maclen /\ disjoint mac m} ->
   aad:uint8_p ->
   aadlen:u32{let len = U32.v aadlen in len = length aad}  ->
-  k:uint8_p{length k = keylen} ->
-  n:uint8_p{length n = noncelen} ->
+  k:uint8_p{length k = keylen /\ (* disjoint k mac /\  *)disjoint k m} ->
+  n:uint8_p{length n = noncelen /\ (* disjoint n mac /\  *)disjoint n m} ->
   Stack u32
-    (requires (fun h -> live h c /\ live h mac /\ live h m /\ live h n /\ live h k))
-    (ensures  (fun h0 z h1 -> modifies_2 c mac h0 h1 /\ live h1 c /\ live h1 mac))
+    (requires (fun h -> live h c /\ live h mac /\ live h m /\ live h n /\ live h k /\ live h aad))
+    (ensures  (fun h0 z h1 -> modifies_1 m h0 h1 /\ live h1 m))
+#reset-options "--initial_fuel 0 --max_fuel 0 --z3rlimit 200"
 let aead_decrypt m c mlen mac aad aadlen k n =
   push_frame();
-  let b = create (uint8_to_sint8 0uy) 64ul in
+  let h0 = ST.get() in
+  let tmp  = create (uint8_to_sint8 0uy) 96ul in
+  let b    = Buffer.sub tmp 0ul 64ul in
+  let lb   = Buffer.sub tmp 64ul 16ul in
+  hstore64_le (Buffer.sub lb 0ul 8ul) (uint32_to_sint64 aadlen);
+  hstore64_le (Buffer.sub lb 8ul 8ul) (uint32_to_sint64 mlen);
+  let rmac = Buffer.sub tmp 80ul 16ul in
   Chacha20.chacha20_key_block b k n 0ul;
   let mk = Buffer.sub b 0ul 32ul in
   let key_s = Buffer.sub mk 16ul 16ul in
-
-  let rmac = create (uint8_to_sint8 0uy) 16ul in
-  let st = Poly1305_64.alloc () in
-  let lb = create (uint8_to_sint8 0uy) 16ul in
-  Poly1305_64.poly1305_blocks_init st aad aadlen mk;
-  Poly1305_64.poly1305_blocks_continue st c mlen;
-  hstore64_le (Buffer.sub lb 0ul 8ul) (uint32_to_sint64 aadlen);
-  hstore64_le (Buffer.sub lb 8ul 8ul) (uint32_to_sint64 mlen);
-  Poly1305_64.poly1305_blocks_finish st lb rmac key_s;
+  aead_encrypt_poly  c mlen rmac aad aadlen k n (Buffer.sub tmp 0ul 80ul);
+  let h1 = ST.get() in
+  cut (modifies_0 h0 h1);
+  (* Declassication assumption on mac *)
+  assume (Hacl.Policies.declassifiable mac /\ Hacl.Policies.declassifiable rmac);
   let verify = cmp_bytes mac rmac 16ul in
-  let res = 
+  let res =
     if U8.(verify =^ 0uy) then (
       	 Chacha20.chacha20 m c mlen k n 1ul;
 	 0ul
   	 ) else 1ul in
+  let h2 = ST.get() in
+  lemma_aead_decrypt h0 h1 h2 tmp m;
   pop_frame();
   res
-
